@prefix rdf:     <http://www.w3.org/1999/02/22-rdf-syntax-ns#> .
@prefix rdfs:    <http://www.w3.org/2000/01/rdf-schema#> .
@prefix rdfg:    <http://www.w3.org/2004/03/trix/rdfg-1/> .
@prefix owl:     <http://www.w3.org/2002/07/owl#> .
@prefix xsd:     <http://www.w3.org/2001/XMLSchema#> .
@prefix cs:      <http://purl.org/vocab/changeset/schema#> .
@prefix fresnel: <http://www.w3.org/2004/09/fresnel#> .
@prefix ordf:    <http://purl.org/NET/ordf/> .
@prefix ordfont: <http://ordf.org/schema/ordf> .
@prefix opmv:    <http://purl.org/net/opmv/ns#> .

ordfont: a owl:Ontology ;
    rdfs:label "ORDF Vocabulary"@en ;
    rdfs:label "Vocabulaire ORDF"@fr ;
    rdfs:comment """The ORDF vocabulary is somewhat of a grab-bag
of predicates that could in principle belong in other vocabularies
but for whatever reason they don't exist.

A major group of predicates is the ones that have to do with 
recording software versions, the host it was run on and such
into an *opmv:Process*.

See the `ORDF Documentation`_ for more information on how and
why these predicates exist.

The canonical namespace for this vocabulary is
http://purl.org/NET/ordf/

.. _ORDF Documentation: http://ordf.org/doc/
""" ;
    rdfs:seeAlso <http://ordf.org/doc/> ;
    rdfs:seeAlso <http://ordf.org/src/> ;
    ordf:lens <http://ordf.org/lens/ontology> .

ordf:version a owl:DatatypeProperty ;
    rdfs:isDefinedBy ordfont: ;
    rdfs:label "ORDF Software Version" ;
    rdfs:comment """Used to record the ORDF software version in an
opmv:Process for provenance purposes. Other packages that wish to
add their versions to provenance information should define a suitable
predicate in their own namespaces as an *rdfs:subPropertyOf* this""" ;
    rdfs:domain opmv:Process .

ordf:cmdline a owl:DatatypeProperty ;
    rdfs:isDefinedBy ordfont: ;
    rdfs:label "Command Line" ;
    rdfs:comment """Used to record the Command line used to operate
on data in an opmv:Process for provenance purposes""" ;
    rdfs:domain opmv:Process .

ordf:pid a owl:DatatypeProperty ;
    rdfs:isDefinedBy ordfont: ;
    rdfs:label "Process ID" ;
    rdfs:comment """Used to record the pid of the process operating on
data in an opmv:Process for provenance purposes""" ;
    rdfs:domain opmv:Process .

ordf:hostname a owl:DatatypeProperty ;
    rdfs:isDefinedBy ordfont: ;
    rdfs:label "Host Name" ;
    rdfs:comment """Used to record the name of the host running a process
operating on data in an opmv:Process for provenance purposes""" ;
    rdfs:domain opmv:Process .

ordf:graph a owl:ObjectProperty ;
    rdfs:isDefinedBy ordfont: ;
    rdfs:label "Reference to a graph" ;
    rdfs:comment """Unfortunately in RDF there is no good way to refer to
an *rdfg:Graph*. This predicate makes that possible.

It is used in particular in the `ORDF extensions`_ to the Talis
*changeset* vocabulary

.. _ORDF extensions: http://ordf.org/doc/changesets.html
""" ;
    rdfs:range rdfg:Graph .

ordf:subGraph a owl:ObjectProperty ;
    rdfs:isDefinedBy ordfont: ;
    rdfs:label "sub-graph" ;
    rdfs:comment """Indicates a sub-graph containing statements belonging
also to this *rdfg:Graph*""" ;
    rdfs:domain rdfg:Graph ;
    rdfs:range rdfg:Graph .

ordf:lens a owl:ObjectProperty ;
    rdfs:isDefinedBy ordfont: ;
    rdfs:label "Lens" ;
    rdfs:comment """Indicates which fresnel:Lens to use when displaying a
graph. In the display system implemented by the *ontosrv* application
the default Fresnel instructions to use to render a *rdfg:Graph* are 
found by looking for this predicate.""" ;
    rdfs:domain rdfg:Graph ;
    rdfs:range fresnel:Lens .

ordf:lensList a owl:ObjectProperty ;
    rdfs:isDefinedBy ordfont: ;
    rdfs:label "Lens List" ;
    rdfs:comment """Indicates the order of applying fresnel:Lens within a
fresnel document. This is an extension to the *fresnel* vocabulary""" .

ordf:changeSet a owl:ObjectProperty ;
    rdfs:isDefinedBy ordfont: ;
    rdfs:label "Change Set" ;
    rdfs:comment """Present in a *rdfg:Graph* to indicate the most recent
changeset in its history""" ;
    rdfs:domain rdfg:Graph ;
    rdfs:range cs:ChangeSet .

ordf:additionCount a owl:DatatypeProperty ;
    rdfs:isDefinedBy ordfont: ;
    rdfs:domain cs:ChangeSet ;
    rdfs:range xsd:integer;
    rdfs:label "Added" ;
    rdfs:comment """Number of statements added in this changeset. This
is an extension to the Talis *changeset* vocabulary""" .

ordf:removalCount a owl:DatatypeProperty ;
    rdfs:isDefinedBy ordfont: ;
    rdfs:domain cs:ChangeSet ;
    rdfs:range xsd:integer;
    rdfs:label "Removed" ;
    rdfs:comment """Number of statements removed in this changeset. This
is an extension to the Talis *changeset* vocabulary""" .
